guard_recursive.cpp: sketch proof
guard_recursive.cpp: Try to break abstractions less

guard_recursive_cpp_proof.v: adapt for new logout interface

guard_recursive_cpp_proof: Drop token and given_token

Sketch alternative derived interfaces

Revised later: instead of dtor_spec'', it's easier to do the proof in C_dtor_ok
with the right hints.

Adapt to derivedR

Proof tweak

C_ctor_spec: higher-level interface

Lift hint

Small cleanups

Generalize hints about Timeless and telescoping functions

Needed to strip laters in next proof.

Move `logout` call from recursive_mutex.dtor_spec'' to C_dtor_ok

Seems a better place in general.

Instances to upstream + improved later-stripping hint

Generalize hint

Automate Inhabited TT

Don't hide TT

rocq-brick-libstdcpp/test/mutex/guard_recursive_cpp_proof.v
@@ -1,9 +1,112 @@
+(** Provisional *)
 Require Import skylabs.auto.cpp.prelude.proof.
 Require Import skylabs.brick.libstdcpp.mutex.spec.
 Require Import skylabs.brick.libstdcpp.test.mutex.guard_recursive_cpp.
 
+Import linearity.
+
+(** TO UPSTREAM START *)
+#[global] Hint Extern 100 (tforall _) => cbn : typeclass_instances.
+Existing Class tforall.
+
+Section to_upstream.
+  #[global] Instance TeleS_inhabited {X : Type} {binder : X → tele} :
+    (∀ x : X, Inhabited (binder x)) →
+    Inhabited X ->
+    Inhabited (TeleS binder).
+  Proof. unshelve solve_inhabited. solve_inhabited. Qed.
+
+  #[global] Instance timeless_tele_app {PROP : bi} {TT : tele} (args : TT) (P : TT -t> PROP):
+    `{(∀.. args, Timeless (tele_app P args)) -> Timeless (tele_app P args)}.
+  Proof.
+    elim: TT args P => [[] //|T TT IH] args P HT.
+    destruct_tele; simpl.
+    apply IH, HT.
+  Qed.
+
+  #[program]
+  Definition strip_timeless_later_is_except_CX {PROP : bi} :=
+    \cancelx
+    \consuming{P : PROP} ▷ P
+    \guard Timeless P
+    \guard{Q} IsExcept0 Q
+    \proving Q
+    \through P -* Q
+    \end.
+  Next Obligation. intros. iIntros ">? ?". work. Qed.
+
+  Section wp_destroy_val.
+    Context `{Σ : cpp_logic, σ : genv}.
+    Context {tu : translation_unit} (cv : type_qualifiers) (ty : type) (p : ptr).
+
+    #[local] Abbreviation WP := (wp_destroy_val tu cv ty p) (only parsing).
+
+    #[global] Instance elim_modal_fupd_wp_destroy_val b P Q :
+      ElimModal True b false (|={top}=> P) P (WP Q) (WP Q).
+    Proof.
+      rewrite /ElimModal. rewrite bi.intuitionistically_if_elim/=.
+      by rewrite fupd_frame_r bi.wand_elim_r fupd_wp_destroy_val.
+    Qed.
+
+    #[global] Instance wp_destroy_val_is_except_0 Q: IsExcept0 (WP Q).
+    Proof.
+      rewrite /IsExcept0 -{2}fupd_wp_destroy_val. by iIntros ">$ !>".
+    Qed.
+  End wp_destroy_val.
+End to_upstream.
+
+#[global] Hint Resolve strip_timeless_later_is_except_CX : br_hints.
+Add Auto Subgoal IsExcept0.
+(** TO UPSTREAM END *)
+
+Implicit Type (p : ptr) (σ : genv).
+
+Abbreviation TT := [tele (_ : Z)].
+Succeed #[global] Instance: Inhabited TT := _.
+
+(** Canonical "constructor" for our telescope. *)
+Polymorphic Definition mk (a : Z) : TT :=
+  {| tele_arg_head := a; tele_arg_tail := () |}.
+Succeed Definition b := recursive_mutex.Held 0 (mk 0).
+
+sl.lock
+Definition CR' `{Σ : cpp_logic, σ : genv} (a : Z) : Rep :=
+  _field "C::value" |-> intR 1$m a.
+#[only(lazy_unfold(export))] derive CR'.
+#[only(timeless)] derive CR'.
+
+sl.lock
+Definition P `{Σ : cpp_logic, σ : genv} (this : ptr) : TT -t> mpred :=
+  fun (a : Z) => this |-> CR' a.
+
+sl.lock
+Definition CR
+  `{Σ : cpp_logic, σ : genv} {HAS_THREADS : HasStdThreads Σ}
+  `{!recursive_mutex.lockedG Σ}
+  `{!HasOwn (iPropI _) recursive_mutex.cmraR}
+  (γ : recursive_mutex.rmutex_gname) (q : cQp.t) :=
+  structR "C" q **
+  _field "C::m" |-> recursive_mutex.derivedR γ q **
+  as_Rep (fun this : ptr =>
+    recursive_mutex.inv_rmutex γ (∃ a : tele_arg TT, tele_app (P this) a)).
+
+#[only(cfractional,ascfractional,cfracvalid,type_ptr)] derive CR.
+#[only(lazy_unfold(export))] derive CR.
+
 Section with_cpp.
   Context `{Σ : cpp_logic, σ : genv} {HAS_THREADS : HasStdThreads Σ}.
+
+  Context `{!recursive_mutex.lockedG Σ}.
+  Context `{!HasOwn (iPropI _) recursive_mutex.cmraR}.
+
+  #[local] Instance: `{WeaklyObjective1 (tele_app (P p))}.
+  Proof. Admitted.
+
+  #[global] Instance P_timeless p a : Timeless (P p a).
+  Proof. rewrite P.unlock; apply _. Qed.
+
+  Succeed #[global] Instance CR'_timeless' p args : Timeless (tele_app (TT := TT) (λ a : Z, p |-> CR' a) args) := _.
+  Succeed #[global] Instance P_timeless' p args : Timeless (tele_app (P p) args) := _.
 
   cpp.spec "test_one_answer()" from source with (
     \post[Vint 42] emp
@@ -12,17 +115,110 @@ Section with_cpp.
     \post[Vint 42] emp
   ).
 
+  Import recursive_mutex(lock_gname).
+
+  cpp.spec "C::C()" from source as C_ctor_spec with (
+    \this this
+    \persist{thr} current_thread thr
+    \post Exists γ,
+      this |-> CR γ 1$m **
+      recursive_mutex.used_threads (lock_gname γ) {[thr]} **
+      recursive_mutex.acquireable (TT := TT) γ thr recursive_mutex.NotHeld (P this)
+  ).
+
+  (** XXX Does not appear to help *)
+  #[global] Instance unfold (p' : ptr) : `{AutoUnlocking.DefinedUsing (P p n) (p' |-> CR' n')} := {}.
+
+  Lemma C_ctor_ok :
+    verify[source] "C::C()".
+  Proof.
+    verify_shift; go.
+    iExists TT, (P this), (mk 0); go.
+    rewrite (* Ugh *) -bi.later_intro.
+    rewrite {1}P.unlock.
+    go.
+
+    iMod (recursive_mutex.use_thread thr (lock_gname t) ∅ with "[$]") as "?"; first set_solver; iModIntro.
+    go.
+    rewrite recursive_mutex.acquireable.unlock (left_id_L _ (∪)).
+    go.
+  Qed.
+
+  cpp.spec "C::~C()" from source as C_dtor_spec with (
+    \this this
+    \persist{thr} current_thread thr
+    \pre{γ} this |-> CR γ 1$m
+    (* \pre recursive_mutex.used_threads (lock_gname γ) empty *)
+    \pre recursive_mutex.used_threads γ.(lock_gname) {[thr]}
+    \pre recursive_mutex.inv_rmutex γ (∃ xs, tele_app (TT := TT) (P this) xs)
+    \pre recursive_mutex.acquireable (TT := TT) γ thr recursive_mutex.NotHeld (P this)
+    \post emp).
+
+  Lemma C_dtor_ok :
+    (* We only get [|> recursive_mutex.dtor_spec'], and that's not enough *)
+    recursive_mutex.dtor_spec' |-- verify[source] "C::~C()".
+  Proof.
+    verify_shift; go.
+    wapply (recursive_mutex.logout thr _ ∅); first by set_solver.
+    rewrite recursive_mutex.acquireable.unlock /= (left_id_L _ (∪)).
+    go with br_erefl.
+    iModIntro.
+    go.
+    progress destruct_tele; rewrite P.unlock /=.
+    go.
+    iApply affine; [apply mpred_BiAffine|go].
+  Qed.
+
+  cpp.spec "C::one_answer()" from source inline.
+
   Lemma test_one_answer_ok :
-    verify?[source] "test_one_answer()".
+    verify[source] "test_one_answer()".
   Proof.
     verify_spec; go.
-  Admitted.
+    destruct args as [a []].
+    rewrite P.unlock /=.
+    go.
+
+    iExists ?[K], (mk 42). go.
+    iSplitL ""; [by go | go].
+    have [? [??]] : exists a, n = 1%nat /\ recursive_mutex.acquire a (recursive_mutex.release (recursive_mutex.Held n (mk 42))). {
+      Unset SsrIdents.
+      rename _n_ into n0.
+      Set SsrIdents.
+      (* This step breaks abstractions, but we have taken the lock yet hints don't
+      give us access to the resouce. *)
+      assert (n0 = 0 /\ n = 1)%nat as [-> ->]. {
+        rewrite-> recursive_mutex.release.unlock in *.
+        destruct n0, n; naive_solver.
+      }
+      rewrite recursive_mutex.release.unlock /=.
+      exists recursive_mutex.NotHeld.
+      split; first done.
+      typeclasses eauto with br_hints.
+    }
+    go.
+    rewrite CR'.unlock.
+    destruct args as [a1 []].
+    go.
+    have [Ha1 Hrel]: (a1 = 42 /\ recursive_mutex.release (recursive_mutex.Held n (mk a1)) = recursive_mutex.NotHeld). {
+      rewrite-> recursive_mutex.release.unlock in *; naive_solver.
+    }
+    subst a1.
+    iExists ?[K], (mk 42). rewrite Hrel /=.
+    go.
+    iSplitL ""; [by go | go].
+    rewrite P.unlock CR'.unlock; go.
+  Qed.
+
+  (* TODO: when we project out equalities about Held and NotHeld, project info
+  about the holding counts; that cancels out better when we repeatedly lock and
+  unlock things. *)
 
   Lemma test_other_answer_ok :
     verify?[source] "test_other_answer()".
   Proof.
     verify_spec; go.
-  Admitted.
+  Abort.
 
   (* WIP, feel free to discard. *)
   (*
